heap/definitions.v
@@ -1,5 +1,9 @@
 Require Import FloydSeq.proofauto.
 Require Import cprogs.heap.program.
+Require Import cprogs.heap.list_relation.
+
+Require Import Coq.micromega.Psatz.
+Require Import SetsClass.SetsClass.
 
 Instance CompSpecs : compspecs. make_compspecs prog. Defined.
 Definition Vprog : varspecs. mk_varspecs prog. Defined.
@@ -12,16 +16,56 @@ Notation "'store_int_array' p l size" :=
   (@data_at CompSpecs Tsh (tarray tint size) (map Vint (map Int.repr l)) p)
   (p at level 0, l at level 0, size at level 0, at level 0).
 
-Parameter MaxHeap : list Z -> Z -> Prop.
-Parameter MaxHeap_p : list Z -> Z -> Z -> Prop.
-Parameter shr : Z -> Z -> Z.
+(* Parameter MaxHeap : list Z -> Z -> Prop. *)
+(* Parameter MaxHeap_p : list Z -> Z -> Z -> Prop. *)
+(* Parameter shr : Z -> Z -> Z. *)
 
-Parameter up : list Z -> Z -> Z -> Z -> list Z.
-Parameter down : list Z -> Z -> Z -> Z -> list Z.
-Parameter push : list Z -> Z -> Z -> list Z.
-Parameter pop : list Z -> Z -> list Z.
-Parameter pop_length : list Z -> Z -> Z.
-Parameter pop_result : list Z -> Z -> Z.
+(* Parameter up : list Z -> Z -> Z -> Z -> list Z. *)
+(* Parameter down : list Z -> Z -> Z -> Z -> list Z. *)
+(* Parameter push : list Z -> Z -> Z -> list Z. *)
+(* Parameter pop : list Z -> Z -> list Z. *)
+(* Parameter pop_length : list Z -> Z -> Z. *)
+(* Parameter pop_result : list Z -> Z -> Z. *)
+
+Definition heap_push: list Z -> Z -> list Z -> Prop :=
+  fun l val l' =>
+    exists (p: Z), heap_list_up (pair (l ++ [val]) (Zlength l)) (pair l' p).
+
+(* Example check_push1: heap_push [233;100;3;2] 5 [233;100;5;2;3].
+Proof.
+  unfold heap_push.
+  exists 2.
+  simpl_Z.
+  apply check_heap_list_up2.
+Qed. *)
+
+Example check_push2: heap_push [233] 400 [233; 400].
+Proof.
+  unfold heap_push.
+  exists 1.
+  simpl_Z.
+  unfold heap_list_up.
+  unfold_RELS_tac.
+  exists O.
+  simpl.
+  unfold list_up_fail.
+  unfold_RELS_tac.
+  simpl fst; simpl snd.
+  try_list_unfold.
+  reflexivity.
+Qed.
+
+Definition heap_pop: list Z -> list Z -> Prop :=
+  fun l l' =>
+    exists (p: Z), heap_list_down (pair (removelast ([Znth 0 l; Znth (Zlength l - 1) l] ++ (skipn 2%nat l))) 1) (pair l' p).
+
+(* Example check_pop1: heap_pop [233;10;6;9;2;4;1;3;4] [233;9;6;4;2;4;1;3].
+Proof.
+  unfold heap_pop.
+  simpl_Z.
+  exists 3.
+  apply check_heap_list_down.
+Qed. *)
 
 Lemma list_length: forall (p: val) (l: list Z) (size: Z),
   !!(size >= 0) && store_int_array p l size |-- !!(Zlength l = size).
@@ -32,7 +76,40 @@ Proof.
   reflexivity.
 Qed.
 
-Print Znth.
+Print firstn.
 
-Lemma MaxHeap_MaxHeap_p : forall l size, MaxHeap l size -> MaxHeap_p l 1 size.
-Proof. Admitted.
+Definition MaxHeap_p (l: list Z) (lo hi: Z): Prop :=
+  forall (i: Z), lo <= i <= hi ->
+    ~(left_son_check_list ((firstn (Z.to_nat (hi + 1)) l), i)) /\ ~(right_son_check_list ((firstn (Z.to_nat (hi + 1)) l), i)).
+
+Definition MaxHeap (l: list Z) (size: Z): Prop :=
+  MaxHeap_p l 1 size.
+
+Definition up: list Z -> Z -> Z -> Z -> list Z -> Prop :=
+  fun l size p0 p1 l' =>
+    heap_list_up ((firstn (Z.to_nat (size + 1)) l), p0) ((firstn (Z.to_nat (size + 1)) l'), p1).
+
+Definition down: list Z -> Z -> Z -> Z -> list Z -> Prop :=
+  fun l size p0 p1 l' =>
+    heap_list_down ((firstn (Z.to_nat (size + 1)) l), p0) ((firstn (Z.to_nat (size + 1)) l'), p1).
+
+Definition push: list Z -> Z -> Z -> list Z -> Prop :=
+  fun l size val l' =>
+    heap_push (firstn (Z.to_nat (size + 1)) l) val (firstn (Z.to_nat (size + 2)) l').
+
+Definition pop: list Z -> Z -> list Z -> Prop :=
+  fun l size l' =>
+    size = 0 /\ l = l' \/ size > 0 /\ heap_pop (firstn (Z.to_nat (size + 1)) l) (firstn (Z.to_nat size) l').
+
+Definition pop_length (l: list Z) (size: Z): Z :=
+  match size with
+    | 0 => 0
+    | _ => size - 1
+  end.
+
+Definition pop_result (l: list Z) (size: Z): Z :=
+  match size with
+    | 0 => -1
+    | _ => 0
+  end.
+
