heap/down/path0.v
@@ -19,12 +19,12 @@ Definition functional_correctness_statement: Prop :=
   forall (Espec: OracleKind) Hl Maxsize size0 pos0 a' pos' size',
   let Delta_specs := Delta_specs_down in
   let Delta := Delta_down Delta_specs in
-  semax Delta (PROP ((MaxHeap_p Hl (Z.add pos0 1) size0); (MaxHeap Hl (Z.sub pos0 1)); (size' = (Vint (IntRepr size0))); (pos' = (Vint (IntRepr pos0))); (Z.le size0 Maxsize); (Z.le 1 size0); (Z.le pos0 size0); (Z.le 1 pos0))
+  semax Delta (PROP ((MaxHeap_p Hl (Z.add pos0 1) size0); (MaxHeap Hl pos0); (size' = (Vint (IntRepr size0))); (pos' = (Vint (IntRepr pos0))); (Z.le size0 Maxsize); (Z.le 1 size0); (Z.le pos0 size0); (Z.le 1 pos0))
   LOCAL (temp _a a'; temp _pos pos'; temp _size size')
   SEP ((store_int_array a' Hl Maxsize)))
   Sskip
   (normal_split_assert
   (EX Hl0 pos1 n a pos size,
-    (PROP ((MaxHeap_p Hl0 (Z.add pos1 1) size0); (MaxHeap Hl0 (Z.sub pos1 1)); (Hl0 = (down Hl size0 pos0 pos1)); (size = (Vint (IntRepr size0))); (pos0 = (shr pos1 n)); (pos = (Vint (IntRepr pos1))); (Z.le pos1 size0))
+    (PROP ((MaxHeap_p Hl0 (Z.add pos1 1) size0); (MaxHeap Hl0 pos1); (down Hl size0 pos0 pos1 Hl0); (size = (Vint (IntRepr size0))); (pos = (Vint (IntRepr pos1))); (Z.le pos1 size0))
     LOCAL (temp _a a; temp _pos pos; temp _size size)
     SEP ((store_int_array a Hl0 Maxsize))))%assert).
