heap/down/path1.v
@@ -20,7 +20,7 @@ Definition functional_correctness_statement: Prop :=
   let Delta_specs := Delta_specs_down in
   let Delta := Delta_down Delta_specs in
   semax Delta (EX Hl0 pos1 n a pos size,
-                (PROP ((MaxHeap_p Hl0 (Z.add pos1 1) size0); (MaxHeap Hl0 (Z.sub pos1 1)); (Hl0 = (down Hl size0 pos0 pos1)); (size = (Vint (IntRepr size0))); (pos0 = (shr pos1 n)); (pos = (Vint (IntRepr pos1))); (Z.le pos1 size0))
+                (PROP ((MaxHeap_p Hl0 (Z.add pos1 1) size0); (MaxHeap Hl0 pos1); (down Hl size0 pos0 pos1 Hl0); (size = (Vint (IntRepr size0))); (pos = (Vint (IntRepr pos1))); (Z.le pos1 size0))
                 LOCAL (temp _a a; temp _pos pos; temp _size size)
                 SEP ((store_int_array a Hl0 Maxsize))))%assert
   (Ssequence
@@ -104,6 +104,6 @@ Definition functional_correctness_statement: Prop :=
                             (Sset _pos (Etempvar _t tint)))))))))))))))
   (normal_split_assert
   (EX Hl0 pos1 n a pos size,
-    (PROP ((MaxHeap_p Hl0 (Z.add pos1 1) size0); (MaxHeap Hl0 (Z.sub pos1 1)); (Hl0 = (down Hl size0 pos0 pos1)); (size = (Vint (IntRepr size0))); (pos0 = (shr pos1 n)); (pos = (Vint (IntRepr pos1))); (Z.le pos1 size0))
+    (PROP ((MaxHeap_p Hl0 (Z.add pos1 1) size0); (MaxHeap Hl0 pos1); (down Hl size0 pos0 pos1 Hl0); (size = (Vint (IntRepr size0))); (pos = (Vint (IntRepr pos1))); (Z.le pos1 size0))
     LOCAL (temp _a a; temp _pos pos; temp _size size)
     SEP ((store_int_array a Hl0 Maxsize))))%assert).
