heap/up/path0.v
@@ -19,12 +19,12 @@ Definition functional_correctness_statement: Prop :=
   forall (Espec: OracleKind) Hl Maxsize size0 pos0 a' pos',
   let Delta_specs := Delta_specs_up in
   let Delta := Delta_up Delta_specs in
-  semax Delta (PROP ((MaxHeap_p Hl (Z.add pos0 1) size0); (MaxHeap Hl (Z.sub pos0 1)); (pos' = (Vint (IntRepr pos0))); (Z.le size0 Maxsize); (Z.le 1 size0); (Z.le pos0 size0); (Z.le 1 pos0))
+  semax Delta (PROP ((MaxHeap_p Hl pos0 size0); (MaxHeap Hl (Z.sub pos0 1)); (pos' = (Vint (IntRepr pos0))); (Z.le size0 Maxsize); (Z.le 1 size0); (Z.le pos0 size0); (Z.le 1 pos0))
   LOCAL (temp _a a'; temp _pos pos')
   SEP ((store_int_array a' Hl Maxsize)))
   Sskip
   (normal_split_assert
   (EX Hl0 pos1 n a pos,
-    (PROP ((MaxHeap_p Hl0 (Z.add pos1 1) size0); (MaxHeap Hl0 (Z.sub pos1 1)); (Hl0 = (up Hl size0 pos0 pos1)); (pos1 = (shr pos0 n)); (pos = (Vint (IntRepr pos1))))
+    (PROP ((MaxHeap_p Hl0 pos1 size0); (MaxHeap Hl0 (Z.sub pos1 1)); (up Hl size0 pos0 pos1 Hl0); (pos = (Vint (IntRepr pos1))))
     LOCAL (temp _a a; temp _pos pos)
     SEP ((store_int_array a Hl0 Maxsize))))%assert).
