heap/up/path2.v
@@ -20,7 +20,7 @@ Definition functional_correctness_statement: Prop :=
   let Delta_specs := Delta_specs_up in
   let Delta := Delta_up Delta_specs in
   semax Delta (EX Hl0 pos1 n a pos,
-                (PROP ((MaxHeap_p Hl0 (Z.add pos1 1) size0); (MaxHeap Hl0 (Z.sub pos1 1)); (Hl0 = (up Hl size0 pos0 pos1)); (pos1 = (shr pos0 n)); (pos = (Vint (IntRepr pos1))))
+                (PROP ((MaxHeap_p Hl0 pos1 size0); (MaxHeap Hl0 (Z.sub pos1 1)); (up Hl size0 pos0 pos1 Hl0); (pos = (Vint (IntRepr pos1))))
                 LOCAL (temp _a a; temp _pos pos)
                 SEP ((store_int_array a Hl0 Maxsize))))%assert
   (Sifthenelse (Ebinop Ogt (Etempvar _pos tint)
@@ -29,6 +29,6 @@ Definition functional_correctness_statement: Prop :=
     Sskip)
   (normal_split_assert (RA_normal (frame_ret_assert (function_body_ret_assert tvoid 
   (EX Hl_final pos1 n a pos,
-    (PROP ((MaxHeap Hl_final size0); (Hl_final = (up Hl size0 pos0 pos1)); (pos1 = (shr pos0 n)); (pos = (Vint (IntRepr pos1))))
+    (PROP ((MaxHeap Hl_final size0); (up Hl size0 pos0 pos1 Hl_final); (pos = (Vint (IntRepr pos1))))
     LOCAL (temp _a a; temp _pos pos)
     SEP ((store_int_array a Hl_final Maxsize))))%assert) (stackframe_of f_up)))).
